---
type: university-assignment
assignment-course: "[[../../../WS24/Logic/Exercise/Exercise|Formal Models (Exercise)]]"
assignment-status: Closed
assignment-deadline: 
---
## Exercise 25
---
### 1
**Consider the formula (c → b) ∧ (c ∨ ¬a) ∧ ((¬c ∨ b) → (c ∨ a)). Find one model σ of φ. What is the value of b? Does a model exist where b has the opposite value?**
   
Using Limboole (Satisfiability check)

input: `(c -> b) & (c | !a) & ((!c | b) -> (c | a))`

output: 
```
% SATISFIABLE formula (satisfying assignment follows)
c = 1
b = 1
a = 0
```

**What is the value of b?**: 
b = 1

**Does a model exist where b has the opposite value?**
b = 0?

Using Limboole (Satisfiability check)

input: `(c -> b) & (c | !a) & ((!c | b) -> (c | a)) & !b`

output: `% UNSATISFIABLE formula`
-> no, a model where b has the opposite value **does not exist.**
### 2
**Apply BCP until fixpoint on the following formula:**

a ∧ (¬a ∨ ¬b) 
∧ (b ∨ ¬a ∨ ¬c) 
∧ (a ∨ ¬d) ∧ (d ∨ c) 
∧ (¬d ∨ g ∨ e ∨ f ) 
∧ (¬g ∨ e ∨ f ) 
∧ (g ∨ ¬e ∨ f ) 
∧ (¬g ∨ ¬e ∨ f )


| Application | BCP                 | formula                                                                                                                                                                       |
| ----------- | ------------------- | ----------------------------------------------------------------------------------------------------------------------------------------------------------------------------- |
| 1           | $BCP(\phi , a)$     | $\neg b \wedge (b \vee\neg c)\wedge (d\vee c)\wedge (\neg d \vee g \vee e \vee f)\wedge (\neg g \vee e\vee f)\wedge (g \vee \neg e \vee f)\wedge (\neg g \vee \neg e \vee f)$ |
| 2           | $BCP(\phi, \neg b)$ | $\neg c \wedge (d\vee c)\wedge(\neg d \vee g \vee e \vee f)\wedge (\neg g \vee e\vee f)\wedge (g \vee \neg e \vee f)\wedge (\neg g \vee \neg e \vee f)$                       |
| 3           | $BCP(\phi, \neg c)$ | $d\wedge (\neg d \vee g \vee e \vee f)\wedge (\neg g \vee e\vee f)\wedge (g \vee \neg e \vee f)\wedge (\neg g \vee \neg e \vee f)$                                            |
| 4           | $BCP(\phi, d)$      | $(g \vee e \vee f)\wedge(\neg g \vee e\vee f)\wedge (g \vee \neg e \vee f)\wedge (\neg g \vee \neg e \vee f)$                                                                 |

**How often and with which literals (l) is BCP applied?**
- it is applied 4 times, with the literals $\{a, \neg b, \neg c, d\}$
**Does an assignment ν exist, that satisfies the formula and ν(c) = 0?**
- Yes, shown in step 2
- Assignment: $\{a, ¬b, ¬c, d, e, f, g\}$
**Does an assignment ν′ exist, that satisfies the formula and ν′( f ) = 0?**
- No, because no matter the assignments of e and g one clause will always be false

## Exercise 26
---
**Given Kripke structure K below. Formulate the transition function as propositional formula.**
![[_attachments/Pasted image 20240516090114.png]]
**Use the naive encoding.**
$\mathcal{T}:= \top$                                           $\wedge$
$(\overline x, \overline y) \rightarrow (\bot \vee (\overline x', y') \vee (x',\overline y'))$       $\wedge$
$(\overline x, y) \rightarrow (\bot \vee (\overline x', \overline y'))$                     $\wedge$
$(x, \overline y) \rightarrow (\bot \vee (x', y') \vee (\overline x', y'))$       $\wedge$ 
$(x, y) \rightarrow (\bot \vee (x', y') \vee (\overline x', y'))$       $\wedge$

**Use the symbolic encoding.**

| <span style="color:#92d050">x</span> | <span style="color:#92d050">y</span> | <span style="color:#9264b4">x'</span> | <span style="color:#9264b4">y'</span> | OR  | <span style="color:#00b0f0">x'</span> | <span style="color:#00b0f0">y'</span> |
| ------------------------------------ | ------------------------------------ | ------------------------------------- | ------------------------------------- | --- | ------------------------------------- | ------------------------------------- |
| 0                                    | 0                                    | 0                                     | 1                                     |     | 1                                     | 0                                     |
| 0                                    | 1                                    | 0                                     | 0                                     |     | 0                                     | 0                                     |
| 1                                    | 0                                    | 1                                     | 1                                     |     | 0                                     | 1                                     |
| 1                                    | 1                                    | 1                                     | 1                                     |     | 0                                     | 1                                     |
$\mathcal{T}:=(x'\leftrightarrow (x) \wedge y' \leftrightarrow (x \vee \overline y))$
$\vee$
$(x'\leftrightarrow (\overline x \wedge \overline y) \wedge y' \leftrightarrow (x))$

## Exercise 27
---
![[_attachments/Pasted image 20240516124659.png]]
**Consider the property p = y. Show that “it is not possible to reach a state that violates p after**
**one step from the initial state” by encoding the problem as a propositional formula. Please**
**encode the entire transition system.**

| <span style="color:#92d050">x</span> | <span style="color:#92d050">y</span> | <span style="color:#9264b4">x'</span> | <span style="color:#9264b4">y'</span> | OR  | <span style="color:#00b0f0">x'</span> | <span style="color:#00b0f0">y'</span> |
| ------------------------------------ | ------------------------------------ | ------------------------------------- | ------------------------------------- | --- | ------------------------------------- | ------------------------------------- |
| 0                                    | 0                                    | 0                                     | 0                                     |     | 0                                     | 0                                     |
| 0                                    | 1                                    | 1                                     | 1                                     |     | 1                                     | 1                                     |
| 1                                    | 0                                    | 1                                     | 0                                     |     | 1                                     | 1                                     |
| 1                                    | 1                                    | 1                                     | 0                                     |     | 1                                     | 0                                     |
$\mathcal{T}:=(x'\leftrightarrow (x \vee (\overline x \wedge y)) \wedge y' \leftrightarrow (\overline x \wedge y))$
$\vee$
$(x'\leftrightarrow (x \vee (\overline x \wedge y)) \wedge y' \leftrightarrow \overline{(x\leftrightarrow y)})$

**In this context, is p a safety, liveness or fairness property?**

<span style="color:#92d050">it's a safety property.</span>

$I(s_0)\wedge\mathcal{T}(s_0,s_1)\wedge B(s_1)$
$\longleftrightarrow$
$(\overline x \wedge y) \wedge  ((x'\leftrightarrow (x \vee (\overline x \wedge y)) \wedge y' \leftrightarrow (\overline x \wedge y))\vee (x'\leftrightarrow (x \vee (\overline x \wedge y)) \wedge y' \leftrightarrow \overline{(x\leftrightarrow y)}))  \wedge \overline y'$

Using limboole: 
input: 
```
(!x0 & y0) 
& (((x-next <-> (x0 | (!x0 & y0))) & (y-next <-> (!x0 & y0))) | ((x-next <-> (x0 | (!x0 & y0))) & (y-next <-> !(x0 <-> y0)))) 
& !y-next
```
output: `% UNSATISFIABLE formula`

**Now show that a state violating p is reachable after two steps. Evaluate your encoding with**
**Limboole.**
Using limboole: 
input: 
```
(!x0 & y0) 
& (((x-next <-> (x0 | (!x0 & y0))) & (y-next <-> (!x0 & y0))) | ((x-next <-> (x0 | (!x0 & y0))) & (y-next <-> !(x0 <-> y0)))) 
& (((x-next-next <-> (x-next | (!x-next & y-next))) & (y-next-next <-> (!x-next & y-next))) | ((x-next-next <-> (x-next | (!x-next & y-next))) & (y-next-next <-> !(x-next <-> y-next)))) 
& !y-next-next
```
output: 
```
% SATISFIABLE formula (satisfying assignment follows)
x0 = 0
y0 = 1
x-next = 1
y-next = 1
x-next-next = 1
y-next-next = 0
```
## Exercise 28
---
**Given the transition function x′ ↔ (¬z) ∧ y′ ↔ (x ∨ y) ∧ z′ ↔ z.**
**Formulate a SAT encoding asking if the safety property x ∧ y is violated after two steps starting**
**from initial states {(x ∧ ¬y ∧ ¬z), (x ∧ ¬y ∧ z)}.** **Is the property violated? Use Limboole to evaluate your encoding.**

Using Limboole:

input:
```
(!x0 & y0)
& ((!x0 & y0)  (x1 & y1)) & ((x0 & y0)  (x1 & !y1)) & ((x0 & !y0) 
((x1 & y1) | (x1 & !y1)))
& ((!x1 & y1)  (x2 & y2)) & ((x1 & y1)  (x2 & !y2)) & ((x1 & !y1) 
((x2 & y2) | (x2 & !y2)))
& !y2
```

output:
```
% SATISFIABLE formula (satisfying assignment follows)
x0 = 0
y0 = 1
x1 = 1
y1 = 1
x2 = 1
y2 = 0
```

The property is violated, as the formula is satisfiable.