---
type: university-assignment
assignment-course: "[[../../../WS24/Logic/Exercise/Exercise|Formal Models (Exercise)]]"
assignment-status: Closed
assignment-deadline: 
---
## Exercise 33
**1. Quantifier prefixes**
- For a true QBF: $\forall a \exists b \exists c \exists d$
- For a false QBF: $\forall a \forall c \exists b \exists d$

**2. Unit Literal Elimination**

> A clause C is called a unit if C contains exactly one existential literal, and the universal literals of C are to the right of the existential literal in the prefix. The existential literal in the unit clause is called the **unit literal ($l$).**

> For Unit Literal Elimination, remove all clauses containing $l$, and remove all occurences of $\bar l$

 $\exists  a  \forall  x  \exists  b  \forall  y  \forall  z  \exists  c  \exists  d.((d)  \wedge  (a  \vee   \neg  c)  \wedge  (x \vee   \neg  c)  \wedge  (a  \vee   \neg  x)  \wedge  (x  \vee   \neg  b  \vee   \neg  y)  \wedge  (  \neg  x  \vee  y\vee   \neg  d)  \wedge (\neg  a  \vee  b \vee z))$

| step | formula                                                                                                                                                                                                                | Unit Clauses           |
| ---- | ---------------------------------------------------------------------------------------------------------------------------------------------------------------------------------------------------------------------- | ---------------------- |
| 0    | $(d)  \wedge  (a  \vee   \neg  c)  \wedge  (x \vee   \neg  c)  \wedge  (a  \vee   \neg  x)  \wedge  (x  \vee   \neg  b  \vee   \neg  y)  \wedge  (  \neg  x  \vee  y\vee   \neg  d)  \wedge (\neg  a  \vee  b \vee z)$ | $(d), (a \vee \neg x)$ |
| 1    | $(x \vee \neg c) \wedge (x \vee \neg b \vee \neg y) \wedge (\neg x \vee y) \wedge (b \vee z)$                                                                                                                          | $(b \vee z)$           |
| 2    | $(x \vee \neg c) \wedge (x \vee \neg y) \wedge (\neg x \vee y)$                                                                                                                                                        | -                      |

## Exercise 34
**1. Pure literal elimination**

>A literal $l$ is pure in a formula $\phi$ if $l$ occurs in $\phi$, and $\bar l$ does not occur in $\phi$.

> For Pure Literal Elimination, remove all clauses with $l$ if $l$ is existentially quantified, and remove all occurences of $l$ if it is universally quantified.

$f=  \exists  a  \forall  x  \exists  b  \forall  y  \exists  c  \forall  z  \exists  d.((a  \vee   \neg  d)  \wedge  (  \neg  a  \vee   \neg  c)  \wedge  (  \neg  y  \vee  z  \vee  d)  \wedge  (  \neg  b  \vee   \neg  z  \vee   \neg  d)  \wedge  (a  \vee  x)  \wedge  (a  \vee  b  \vee  y))$

| step | formula                                                                                                                                                                                                     | Pure literals    |
| ---- | ----------------------------------------------------------------------------------------------------------------------------------------------------------------------------------------------------------- | ---------------- |
| 0    | $(a  \vee   \neg  d)  \wedge  (  \neg  a  \vee   \neg  c)  \wedge  (  \neg  y  \vee  z  \vee  d)  \wedge  (  \neg  b  \vee   \neg  z  \vee   \neg  d)  \wedge  (a  \vee  x)  \wedge  (a  \vee  b  \vee  y)$ | $x, \neg c$      |
| 1    | $(a  \vee   \neg  d) \wedge  (  \neg  y  \vee  z  \vee  d)  \wedge  (  \neg  b  \vee   \neg  z  \vee   \neg  d)  \wedge  a  \wedge  (a  \vee  b  \vee  y)$                                                  | $a$              |
| 2    | $(  \neg  y  \vee  z  \vee  d)  \wedge  (  \neg  b  \vee   \neg  z  \vee   \neg  d)$                                                                                                                        | $\neg b, \neg y$ |
| 3    | $(z  \vee  d)$                                                                                                                                                                                              | $z, d$           |
| 4    | $() \rightarrow \top$                                                                                                                                                                                       | -                |

**2. Apply universal reduction to $g$**

>If there is no existential prefixed literal ($\exists$) to the right of a universal literal ($\forall$), then we can remove it. Literals must be ordered first.

$g = \forall x \exists a \forall y \exists b \forall z \exists c \forall w \exists d.((\neg a \vee y \vee b) \wedge (a \vee y \vee w) \wedge (b \vee z \vee w) \wedge (\neg x \vee w \vee d) \wedge (x \vee \neg c \vee \neg w))$

| step  | g                                                                                                                                           |
| ----- | ------------------------------------------------------------------------------------------------------------------------------------------- |
| 0     | $(\neg a \vee y \vee b) \wedge (a \vee y \vee w) \wedge (b \vee z \vee w) \wedge (\neg x \vee w \vee d) \wedge (x \vee \neg c \vee \neg w)$ |
| 1 (w) | $(\neg a \vee y \vee b) \wedge (a \vee y) \wedge (b \vee z) \wedge (\neg x \vee w \vee d) \wedge (x \vee \neg c)$                           |
| 2 (z) | $(\neg a \vee y \vee b) \wedge (a \vee y) \wedge (b) \wedge (\neg x \vee w \vee d) \wedge (x \vee \neg c)$                                  |
| 3 (y) | $(\neg a \vee y \vee b) \wedge (a) \wedge (b) \wedge (\neg x \vee w \vee d) \wedge (x \vee \neg c)$                                         |
## Exercise 35
**Use the splitting algorithm from the lecture slides to determine the truth value of the following
formula:**

```
boolean splitCNF (Prefix P, matrix ψ)
if (ψ == ∅): return true;
if (∅ ∈ ψ): return false;

P = QXP', x ∈ X, X = X\{x};

if (Q == ∀)
    return(splitCNF(QX'P', ψ') && 
          splitCNF(QX'P', ψ''));
else
    return(splitCNF(QX'P', ψ') ||
           splitCNF(QX'P', ψ''));

where:
ψ': take clauses of ψ, delete clauses with x, delete ¬x
ψ'': take clauses of ψ, delete clauses with ¬x, delete x
```

$\exists  a  \forall  x  \exists  b  \forall  y  \exists  c.((a  \vee  x  \vee  y  \vee  c)  \wedge  (a  \vee  y)  \wedge  (  \neg  x  \vee  b)  \wedge  (  \neg  a  \vee   \neg  y  \vee   \neg  b)  \wedge  (b  \vee   \neg  c)  \wedge  (x  \vee  y  \vee  c))$

OR from  $\exists a$, $((a  \vee  x  \vee  y  \vee  c)  \wedge  (a  \vee  y)  \wedge  (  \neg  x  \vee  b)  \wedge  (  \neg  a  \vee   \neg  y  \vee   \neg  b)  \wedge  (b  \vee   \neg  c)  \wedge  (x  \vee  y  \vee  c))$ -----> $\bot$
- AND from $\forall x$, $((  \neg  x  \vee  b)  \wedge  (\neg  y  \vee   \neg  b)  \wedge  (b  \vee   \neg  c)  \wedge  (x  \vee  y  \vee  c))$ ----> $\bot$
	- OR from $\exists b$, $((b)  \wedge  (\neg  y  \vee   \neg  b)  \wedge  (b  \vee   \neg  c))$ ---> $\bot$
		- AND from $\forall y, ((\neg y))$ --> $\bot$
			- RETURN (()) -> $\bot$
			- RETURN () -> $\top$
		- RETURN $(() \wedge (\neg c))$ --> $\bot$
	- OR from $\exists b$, $((\neg  y  \vee   \neg  b)  \wedge  (b  \vee   \neg  c)  \wedge  (y  \vee  c))$
		- ... don't need to evaluate, above OR is already false, making the AND statement false
- AND from $\forall x$, $((x  \vee  y  \vee  c)  \wedge  (y)  \wedge  (  \neg  x  \vee  b)  \wedge (b  \vee   \neg  c)  \wedge  (x  \vee  y  \vee  c))$ ----> $\bot$
	- OR from $\exists b$, $((y)  \wedge  (b)  \wedge (b  \vee   \neg  c))$ ---> $\bot$
		- AND from $\forall y, ((y))$ --> $\bot$
			- RETURN $()$ -> $\top$
			- RETURN (()) -> $\bot$
		- RETURN $\forall y, ((y) \wedge () \wedge (\neg c))$ -> $\bot$
	- OR from $\exists b$, $(y  \vee  c)  \wedge  y  \wedge (b  \vee   \neg  c)  \wedge  (y  \vee  c)$
		- ... no point in evaluating, above OR is already false, making the AND statement false

The formula is false.
## Exercise 36
**1. Is there a path of length 7 (exactly 7 transitions) from A to D?**

from UE07:
$\mathcal{T}:=(x'\leftrightarrow (x) \wedge y' \leftrightarrow (x \vee \overline y))$
$\vee$
$(x'\leftrightarrow (\overline x \wedge \overline y) \wedge y' \leftrightarrow (x))$

Limboole input:
```Limboole
% existential variables
?x0 ?y0 ?x1 ?y1 ?x2 ?y2 ?x3 ?y3 ?x4 ?y4 ?x5 ?y5 ?x6 ?y6 ?x7 ?y7

% universally quantifiable
#x #y #x-next #y-next

% initial state
!x0 & !y0 &

% final state
x7 & y7 &

((
	(x <-> x0) & (y <-> y0) & (x-next <-> x1) & (y-next <-> y1) |
	(x <-> x1) & (y <-> y1) & (x-next <-> x2) & (y-next <-> y2) |
	(x <-> x2) & (y <-> y2) & (x-next <-> x3) & (y-next <-> y3) |
	(x <-> x3) & (y <-> y3) & (x-next <-> x4) & (y-next <-> y4) |
	(x <-> x4) & (y <-> y4) & (x-next <-> x5) & (y-next <-> y5) |
	(x <-> x5) & (y <-> y5) & (x-next <-> x6) & (y-next <-> y6) |
	(x <-> x6) & (y <-> y6) & (x-next <-> x7) & (y-next <-> y7)
) -> (
	((x-next <-> x) & (y-next <-> (x | !y))) |
	((x-next <-> (!x & !y)) & (y-next <-> x))
))
```

Limboole output:
```
% TRUE FORMULA (satisfying assignment of outermost existential variables follows)
x0 = 0
y0 = 0
x1 = 0
y1 = 1
x2 = 0
y2 = 0
x3 = 1
y3 = 0
x4 = 0
y4 = 1
x5 = 0
y5 = 0
x6 = 1
y6 = 0
x7 = 1
y7 = 1
```
Yes, there is such a path.

**2. Is there such a path where additionally ¬x holds in the first 4 states of the path?**

```
% existential variables
?x0 ?y0 ?x1 ?y1 ?x2 ?y2 ?x3 ?y3 ?x4 ?y4 ?x5 ?y5 ?x6 ?y6 ?x7 ?y7

% universally quantifiable
#x #y #x-next #y-next

% initial state
!x0 & !y0 &

% final state
x7 & y7 &

% !x should hold in the first 4 states
!x0 & !x1 & !x2 & !x3 &

((
	(x <-> x0) & (y <-> y0) & (x-next <-> x1) & (y-next <-> y1) |
	(x <-> x1) & (y <-> y1) & (x-next <-> x2) & (y-next <-> y2) |
	(x <-> x2) & (y <-> y2) & (x-next <-> x3) & (y-next <-> y3) |
	(x <-> x3) & (y <-> y3) & (x-next <-> x4) & (y-next <-> y4) |
	(x <-> x4) & (y <-> y4) & (x-next <-> x5) & (y-next <-> y5) |
	(x <-> x5) & (y <-> y5) & (x-next <-> x6) & (y-next <-> y6) |
	(x <-> x6) & (y <-> y6) & (x-next <-> x7) & (y-next <-> y7)
) -> (
	((x-next <-> x) & (y-next <-> (x | !y))) |
	((x-next <-> (!x & !y)) & (y-next <-> x))
))
```

Limboole output:
```
% TRUE FORMULA (satisfying assignment of outermost existential variables follows)
x0 = 0
y0 = 0
x1 = 0
y1 = 1
x2 = 0
y2 = 0
x3 = 0
y3 = 1
x4 = 0
y4 = 0
x5 = 1
y5 = 0
x6 = 1
y6 = 1
x7 = 1
y7 = 1
```
Yes, such a path still exists.

**3. Is there a path of length 6 from A to C where ¬x holds in every state except for the last one?**

```
% existential variables
?x0 ?y0 ?x1 ?y1 ?x2 ?y2 ?x3 ?y3 ?x4 ?y4 ?x5 ?y5 ?x6 ?y6

% universally quantifiable
#x #y #x-next #y-next

% initial state
!x0 & !y0 &

% final state
x6 & !y6 &

% !x should hold in all states except the last
!x0 & !x1 & !x2 & !x3 & !x4 & !x5 &

((
	(x <-> x0) & (y <-> y0) & (x-next <-> x1) & (y-next <-> y1) |
	(x <-> x1) & (y <-> y1) & (x-next <-> x2) & (y-next <-> y2) |
	(x <-> x2) & (y <-> y2) & (x-next <-> x3) & (y-next <-> y3) |
	(x <-> x3) & (y <-> y3) & (x-next <-> x4) & (y-next <-> y4) |
	(x <-> x4) & (y <-> y4) & (x-next <-> x5) & (y-next <-> y5) |
	(x <-> x5) & (y <-> y5) & (x-next <-> x6) & (y-next <-> y6)
) -> (
	((x-next <-> x) & (y-next <-> (x | !y)))) |
	((x-next <-> (!x & !y)) & (y-next <-> x))
))
```

```
% FALSE formula
```
No such path exists.

${a \over b} = {\frac{a}{b}}$
